update

EncRelSeq/MonadsAsHigh/AbsMonad/encimpmonad.v
@@ -1,7 +1,11 @@
+
+From AUXLib Require Import List_lemma.
 From SetsClass Require Import SetsClass.
-From EncRelSeq.Basics Require Import basictacs basicasrt relasrt encdefs relhoarelogic safeexec_lib.
-From EncRelSeq.UBError Require Import errsem hoarelogic relhoarelogic safeexec_lib.
-From EncRelSeq Require Import callsem contexthoare contexthoare_imp. 
+From EncRelSeq.Basics Require Import basictacs basicasrt relasrt encdefs.
+From EncRelSeq.Functioncall Require Import callsem contexthoare contexthoare_imp.
+From EncRelSeq.MonadsAsHigh.AbsMonad Require Import relhoarelogic encrel.
+Require Import MonadLib.MonadLib.
+Import StateRelMonad.
 Require Import Coq.Lists.List.
 Require Import Coq.ZArith.ZArith.
 From AUXLib Require Import Idents .
@@ -11,76 +15,69 @@ Local Open Scope sets.
 
 (*************************************************************************************************************)
 (**********************************   Encode contextual relational triples   *********************************)
-(**********************************             including errors             *********************************)
 (**********************************   High-level setting                     *********************************)
-(**********************************          1. high denosem  no  call       *********************************)
+(**********************************          1. monad  no error              *********************************)
 (*************************************************************************************************************)
-Module RelJoinStateGlobalEnvHighNoCall.
+Module RelImpAbsMonad.
 
 Import practicaldeno.
-Import RelHoarePracticalDeno.
-Import PracticalDenoConstructs.
-Import HoarePracticalDeno.
-Import ContextualJoinStateGlobalEnv.
-
+Import RelHoareNormalDenoAsbMonad2.
+Import NormalContextualImp.
+(* Import EncNormalDenoAbsMonad. *)
 Section contextual_relationaltriples.
   Context {lgst : lgstate}.
   Context {callc: @calllang_envstate local_cstate global_cstate}.
 
   Context {Σₕ: Type}.
 
-  Definition relassertion := @relasrt local_cstate Σₕ (@denosem Σₕ).
-  Record relfuncspec : Type := mk_relfuncspec {
+  Definition relassertion {A: Type}:= @relasrt local_cstate Σₕ (program Σₕ A).
+  Record relfuncspec  : Type := mk_relfuncspec {
+    rA: Type;
     rFS_With : Type;
-    rFS_Pre : rFS_With -> relassertion;
-    rFS_Post : rFS_With -> relassertion;
+    rFS_Pre : rFS_With -> @relassertion rA;
+    rFS_Post : rFS_With -> @relassertion rA;
   }.
 
   (* funcspecs_sat *)
 
   Definition relfuncspecs : Type := list (func * relfuncspec).
 
-  Definition relfuncspecs_sat (χ : func -> @denosem global_cstate)
+  Definition relfuncspecs_sat (χnrm : (func -> global_cstate -> global_cstate -> Prop))
                         (Gamma : relfuncspecs) : Prop :=
     forall f fspec,
     In (f, fspec) Gamma -> 
     forall (w : fspec.(rFS_With)) lst1 lm1 lmf hst1 hstmt,
       join lm1 lmf lst1.(st_mem) ->
       fspec.(rFS_Pre) w ((mk_lstate lst1.(lenv) lst1.(genv) lm1), hst1, hstmt) ->
-      ((χ f).(err) (mk_gstate lst1.(genv) lst1.(st_mem))  -> (hstmt).(err) hst1) /\
       forall lgst2, 
-        (χ f).(nrm) (mk_gstate lst1.(genv) lst1.(st_mem)) lgst2 -> ((hstmt).(err) hst1) \/
+        (χnrm f) (mk_gstate lst1.(genv) lst1.(st_mem)) lgst2 -> 
         exists hst2 hstmt2, 
         ( hst1, hstmt ) ↪ ( hst2, hstmt2 ) /\
         exists lm2, join lm2 lmf lgst2.(gst_mem) /\
         fspec.(rFS_Post) w ((mk_lstate lst1.(lenv) lgst2.(ggenv) lm2), hst2, hstmt2).
 
-  Definition valid_reltriple  (χ : func -> @denosem global_cstate) :=
+  Definition valid_reltriple {A: Type} (χnrm : (func -> global_cstate -> global_cstate -> Prop)) :=
     fun (P : relassertion) (c : Langstmts) (Q : relassertion) =>
-    forall lst1 lm1 lmf hst1 hstmt1, join lm1 lmf lst1.(st_mem) -> P ((mk_lstate lst1.(lenv) lst1.(genv) lm1), hst1, hstmt1) ->  
-            ((evalerr (fun f => (χ f).(nrm)) (fun f => (χ f).(err)) c) lst1  ->  
-            (hstmt1).(err) hst1) /\ 
-    forall lst2, (evalnrm (fun f => (χ f).(nrm)) c) lst1 lst2 ->
-    ((hstmt1).(err) hst1) \/
+    forall lst1 lm1 lmf hst1 (hstmt1: program Σₕ A), join lm1 lmf lst1.(st_mem) -> P ((mk_lstate lst1.(lenv) lst1.(genv) lm1), hst1, hstmt1) ->  
+    forall lst2, (evalnrm (χnrm) c) lst1 lst2 ->
     exists hst2 hstmt2, 
     ( hst1, (hstmt1) ) ↪ ( hst2, (hstmt2) ) /\
     exists lm2, join lm2 lmf lst2.(st_mem) /\
     Q ((mk_lstate lst2.(lenv) lst2.(genv) lm2), hst2, hstmt2).
 
 
-  Definition valid_contextualreltriple (Delta : funcspecs) (Gamma : relfuncspecs)  :=
+  Definition valid_contextualreltriple {A: Type} (Delta : funcspecs) (Gamma : relfuncspecs)  :=
     fun  (P : relassertion) (c : Langstmts) (Q : relassertion) =>
     forall χ,
-    funcspecs_sat χ Delta ->  relfuncspecs_sat χ Gamma ->
-    valid_reltriple χ P c Q.
+    funcspecs_sat_nrm χ Delta ->  relfuncspecs_sat χ Gamma ->
+    @valid_reltriple A χ P c Q.
 
-  Lemma relfuncspecs_equivforall : forall Γ χ ,
-    relfuncspecs_sat χ Γ <-> Forall (fun '(f, fspec) => forall (w : fspec.(rFS_With)) lst1 lm1 lmf hst1 hstmt,
+  Lemma relfuncspecs_equivforall : forall Γ χnrm ,
+    relfuncspecs_sat χnrm Γ <-> Forall (fun '(f, fspec) => forall (w : fspec.(rFS_With)) lst1 lm1 lmf hst1 hstmt,
     join lm1 lmf lst1.(st_mem) ->
     fspec.(rFS_Pre) w ((mk_lstate lst1.(lenv) lst1.(genv) lm1), hst1, hstmt) ->
-    ((χ f).(err) (mk_gstate lst1.(genv) lst1.(st_mem))  -> (hstmt).(err) hst1) /\
     forall lgst2, 
-      (χ f).(nrm) (mk_gstate lst1.(genv) lst1.(st_mem)) lgst2 -> ((hstmt).(err) hst1) \/
+      (χnrm f)(mk_gstate lst1.(genv) lst1.(st_mem)) lgst2 ->
       exists hst2 hstmt2, 
       ( hst1, hstmt ) ↪ ( hst2, hstmt2 ) /\
       exists lm2, join lm2 lmf lgst2.(gst_mem) /\
@@ -108,7 +105,7 @@ Section encode_contextual_triples.
 
 
   Definition encode_relfuncspec (rfspec: relfuncspec) : funcspec :=
-    mk_funcspec ((Σₕ -> Prop) * rfspec.(rFS_With)) 
+    mk_funcspec ((rfspec.(rA) -> Σₕ -> Prop) * rfspec.(rFS_With)) 
                 (fun '(X, w) => encode_asrt (rfspec.(rFS_Pre) w) X) 
                 (fun '(X, w) => encode_asrt (rfspec.(rFS_Post) w) X). 
 
@@ -118,9 +115,9 @@ Section encode_contextual_triples.
     | (fid, rfspec) :: Gamma' =>  (fid, encode_relfuncspec rfspec) :: (encode_relfuncspecs Gamma')
     end.
 
-  Definition valid_contextualrelT (Delta : funcspecs) (Gamma : relfuncspecs) 
-    (P: @relasrt local_cstate Σₕ (@denosem Σₕ)) (cₗ: Langstmts) (Q : @relasrt local_cstate Σₕ (@denosem Σₕ)) := 
-      forall X, valid_contextualtriple (Delta ++ (encode_relfuncspecs Gamma))
+  Definition valid_contextualrelT {A: Type} (Delta : funcspecs) (Gamma : relfuncspecs) 
+    (P: @relasrt local_cstate Σₕ (program Σₕ A)) (cₗ: Langstmts) (Q : @relasrt local_cstate Σₕ (program Σₕ A)) := 
+      forall X, valid_contextualtriple_nrm   (Delta ++ (encode_relfuncspecs Gamma))
                         (encode_asrt P X)
                         cₗ 
                         (encode_asrt Q X).
@@ -133,8 +130,6 @@ Notation " '(|' Γ '|)'  " := (encode_relfuncspecs Γ)  (at level 20, no associa
 (*************************************************************************************************************)
 (*******************************     soundness proof for valid_contextualrelT    *****************************)
 (*************************************************************************************************************)
-Import Coq.Logic.Classical_Prop.
-
 Section contextual_validity_soundness.
   Context {lgst : lgstate}.
   Context {callc: @calllang_envstate local_cstate global_cstate}.
@@ -144,71 +139,52 @@ Section contextual_validity_soundness.
   Local Notation " Δ ⩅ Γ '⊢' '⟨' P '⟩' c '⟨' Q '⟩'" := (valid_contextualreltriple Δ Γ P c Q) (at level 71, no associativity).
   Local Notation " Δ ⩅ Γ '⊢ₑ' '⟨' P '⟩' c '⟨' Q '⟩'" := (valid_contextualrelT Δ Γ P c Q) (at level 71, no associativity).
 
-
-  Lemma funcspecs_equiv_relfuncspecs:  forall (Γ : relfuncspecs) (χ: func -> denosem),
-    funcspecs_sat χ (@encode_relfuncspecs lgst Σₕ Γ) <-> 
-    relfuncspecs_sat χ Γ.
+  Lemma funcspecs_equiv_relfuncspecs:  forall (Γ : relfuncspecs) (χnrm: (func -> global_cstate -> global_cstate -> Prop)),
+    funcspecs_sat_nrm χnrm (@encode_relfuncspecs lgst Σₕ Γ) <-> 
+    relfuncspecs_sat χnrm Γ.
   Proof.
     induction Γ;intros.
     - split;intros. 
       apply relfuncspecs_equivforall. constructor.
-      cbn. apply funcspecs_equivforall. constructor.
+      cbn. apply funcspecs_nrm_equivforall. constructor.
     - split;intros.
       { apply relfuncspecs_equivforall.
       destruct a as [f fspec].
       cbn in H.
-      apply funcspecs_equivforall in H.
+      apply funcspecs_nrm_equivforall in H.
       inversion H. subst.
       clear H.
       constructor;auto.
       + clear H3.
-        intros.
-        destruct fspec as [rfwith RP RQ].
+        intros * H H1.
+        destruct fspec as [A rfwith RP RQ].
         cbn in *.
-        remember (fun hst => (hstmt).(nrm) hst1 hst) as X.
+        remember (fun r hst => (hstmt) hst1 r hst) as X.
         specialize (H2 lst1 lm1 lmf (X, w) H).
         cbn in H2.
-        split.
-        * intros.
-          pose proof classic ((hstmt).(err) hst1) as [ | ];[auto | ].
+          intros * HLeval.
           assert (encode_asrt (RP w) X {| lenv := lenv lst1; genv := genv lst1; st_mem := lm1 |}).
           { unfold encode_asrt.
             do 2 eexists.
             split;eauto.
-            unfold safe.
-            split;auto.
+            simpl_hdefs. unfold weakestpre. sets_unfold.
             intros.
             subst X.
             auto.
           }
-          specialize (H2 H4) as [? _].
-          contradiction.
-        * intros * HLeval.
-          pose proof classic ((hstmt).(err) hst1) as [HHerr | HHnerr];[auto | ].
-          right.
-          assert (encode_asrt (RP w) X {| lenv := lenv lst1; genv := genv lst1; st_mem := lm1 |}).
-          { unfold encode_asrt.
-            do 2 eexists.
-            split;eauto.
-            split;auto.
-            intros.
-            subst X.
-            auto.
-          }
-          specialize (H2 H1) as [_ ?].
+          specialize (H2 H0) as H2.
           specialize (H2 _ HLeval).
           unfold encode_asrt in H2.
-          destruct H2 as (lm2 & Hjoin & hst2 & hstmt2 & [? ?] & HQ).
+          destruct H2 as (lm2 & Hjoin & hst2 & hstmt2 & ? & HQ).
           do 2 eexists.
           split;eauto.
           unfold config_refinement.
-          split;intros.
-          { subst X. eapply H3;eauto. }  
-          contradiction.
+          intros.
+          subst X. eapply H2;eauto.
       + apply relfuncspecs_equivforall.
         apply IHΓ.
-        apply funcspecs_equivforall;auto. }
-      apply funcspecs_equivforall.
+        apply funcspecs_nrm_equivforall;auto.  }
+      apply funcspecs_nrm_equivforall.
       destruct a as [f fspec].
       cbn.
       apply relfuncspecs_equivforall in H.
@@ -216,116 +192,83 @@ Section contextual_validity_soundness.
       clear H.
       constructor;auto.
       + clear H3.
-        intros.
+        intros * H H0.
         destruct fspec as [fwith P Q].
         cbn in *.
         destruct w as [X w].
-        destruct H0 as (hst1 & hstmt & [HHerr HHnrm] & HP).
-        specialize (H2 w _ _ _  hst1 hstmt H HP) as [Herr Hnrm].
-        split.
-        * intros.
-          unfold not.
-          intros.
-          apply HHerr. intuition auto.
-        * intros * HLeval.
+        destruct H0 as (hst1 & hstmt & HHnrm & HP).
+        specialize (H2 w _ _ _  hst1 hstmt H HP) as  Hnrm.
+          intros * HLeval.
           specialize (Hnrm _ HLeval).
-          destruct Hnrm.
-          contradiction.
-          destruct H0 as (hst2 & hstmt2 & [Hheval1 Hheval2] & (lm2 & ? & ?)).
+          destruct Hnrm as (hst2 & hstmt2 & Hheval & (lm2 & ? & ?)).
           eexists.
           split;eauto.
           exists hst2, hstmt2.
           split;auto.
-          split;auto.
-      + apply funcspecs_equivforall.
+          simpl_hdefs. unfold weakestpre. sets_unfold. auto.
+      + apply funcspecs_nrm_equivforall.
         apply IHΓ.
         apply relfuncspecs_equivforall;auto.
   Qed.
 
-  Theorem encoding_correctness : forall (Δ : funcspecs) (Γ : relfuncspecs) (P: @relasrt local_cstate Σₕ (@denosem Σₕ)) (cₗ: Langstmts) 
-    (Q : @relasrt local_cstate Σₕ (@denosem Σₕ)),
+  Theorem encoding_correctness {A: Type}: forall (Δ : funcspecs) (Γ : relfuncspecs) (P: @relasrt local_cstate Σₕ (program Σₕ A)) (cₗ: Langstmts) 
+    (Q : @relasrt local_cstate Σₕ (program Σₕ A)),
     Δ ⩅ Γ  ⊢ ⟨ P ⟩ cₗ ⟨ Q ⟩ <-> Δ ⩅ Γ ⊢ₑ ⟨ P ⟩ cₗ ⟨ Q ⟩.
   Proof.
     intros;split.
-    - unfold valid_contextualreltriple, valid_contextualrelT, valid_contextualtriple.
+    - unfold valid_contextualreltriple, valid_contextualrelT, valid_contextualtriple_nrm.
       intros HT X χ HDelta lst1 lm1 lmf Hframe HP. 
-      apply funcspecs_sat_app in HDelta as [HDelta HGamma].
+      apply funcspecs_sat_nrm_app in HDelta as [HDelta HGamma].
       apply funcspecs_equiv_relfuncspecs in HGamma.
       specialize (HT _ HDelta HGamma).
       unfold valid_reltriple in HT.
       unfold encode_asrt in HP.
-      destruct HP as (hst1 & hstmt1 & [Hherr Hhnrm] & HP).
-      specialize (HT _ _ _ _ _ Hframe HP) as [Herr Hnrm].
-      split.
-      + unfold not in *. intros. apply Hherr. intuition auto.
-      +  
+      destruct HP as (hst1 & hstmt1 & Hhnrm & HP).
+      specialize (HT _ _ _ _ _ Hframe HP) as  Hnrm.
       intros lst2 Heval.
       unfold encode_asrt.
-      specialize (Hnrm _ Heval) as [ | (hst2 & hstmt2 & [Hheval Hhevalerr] & lm2 & Hframe2 & HQ) ];[contradiction | ].
+      specialize (Hnrm _ Heval) as (hst2 & hstmt2 & Hheval & lm2 & Hframe2 & HQ).
       eexists.
       split;eauto.
-      do 2 eexists. split;eauto.
-      unfold safe.
-      split;[cbn;auto | ].
-      cbn;intros.
+      do 2 eexists. split;[ | eauto].
+      simpl_hdefs. unfold weakestpre. sets_unfold.
+      intros.
       sets_unfold in H. subst.
       eapply Hhnrm;eauto.
-    - unfold valid_contextualreltriple, valid_contextualrelT, valid_contextualtriple.
+    - unfold valid_contextualreltriple, valid_contextualrelT, valid_contextualtriple_nrm.
       intros HT χ HDelta HGamma lst1 lm1 lmf hst1 hstmt1 Hframe HP.
-      specialize (HT (fun hst => (hstmt1).(nrm) hst1 hst) χ).
-      assert (funcspecs_sat χ (Δ ++ encode_relfuncspecs Γ)).
-      { apply funcspecs_sat_app.
+      specialize (HT (fun r hst => (hstmt1) hst1 r  hst) χ).
+      assert (funcspecs_sat_nrm χ (Δ ++ encode_relfuncspecs Γ)).
+      { apply funcspecs_sat_nrm_app.
         split;auto.
         apply funcspecs_equiv_relfuncspecs.
         auto. 
       }
       specialize (HT H lst1 _ _ Hframe).
-      split.
-      + intros.
-        (* excluded middle used *)
-        pose proof classic (err (hstmt1) hst1) as [ | ];[auto | ].
-        assert (encode_asrt P (fun hst : Σₕ => nrm hstmt1 hst1 hst)
-        {| lenv := lenv lst1; genv := genv lst1; st_mem := lm1 |}).
-        { unfold encode_asrt.
-          do 2 eexists. split;eauto.
-          split;auto. 
-        }
-        specialize (HT H2) as [? ?].
-        contradiction.
-      + intros lst2 Heval.
-        (* excluded middle used *)
-        pose proof classic (err (hstmt1) hst1) as [ | ];[auto | ].
-        right.
-        assert (encode_asrt P (fun hst : Σₕ => nrm hstmt1 hst1 hst)
+        intros lst2 Heval.
+        assert (encode_asrt P (fun (r : A) (hst : Σₕ) => hstmt1 hst1 r hst)
         {| lenv := lenv lst1; genv := genv lst1; st_mem := lm1 |}).
         { unfold encode_asrt, lift.
           do 2 eexists. split;eauto.
-          split;auto. 
+          simpl_hdefs. unfold weakestpre. sets_unfold.
+          intros;auto. 
         }
-        specialize (HT H1) as [? ?].
-        specialize (H3 _ Heval) as (lm2 & Hframe2 & H3). 
-        unfold encode_asrt in H3.
-        destruct H3 as [hst2 [hstmt2 [? ?]]];subst.
+        specialize (HT H0) as ?.
+        specialize (H1 _ Heval) as (lm2 & Hframe2 & H2). 
+        unfold encode_asrt in H2. simpl_hdefs. 
+        destruct H2 as [hst2 [hstmt2 [? ?]]];subst.
         do 2 eexists.
         split;eauto.
-        unfold config_refinement;cbn.
-        split.
-        { intros. 
-        unfold safe in H3.
-        destruct H3 as [_ ?].
-        sets_unfold in H3.
-        auto. }
-        intros.
-        unfold safe in H3.
-        destruct H3 as [? _].
-        contradiction.
+        unfold weakestpre in *. sets_unfold in H1.
+        unfold config_refinement.
+        apply H1.
   Qed. 
   
 End contextual_validity_soundness.
+
 Local Open Scope asrt_scope. 
 Notation " Δ ⩅ Γ '⊢' '⟨' P '⟩' c '⟨' Q '⟩'" := (valid_contextualreltriple Δ Γ P c Q) (at level 71, no associativity).
 Notation " Δ ⩅ Γ '⊢ₑ' '⟨' P '⟩' c '⟨' Q '⟩'" := (valid_contextualrelT Δ Γ P c Q) (at level 71, no associativity).
-
 (**********************************************************************************)
 (*    encode asrt rules                                                           *)
 (**********************************************************************************)
@@ -335,8 +278,8 @@ Section  SepRAssertion.
   
   Context {Σₕ: Type}.
 
-  Definition relexpr : Type := local_cstate * Σₕ * (@denosem Σₕ).
-  Definition rjoin : (relexpr) -> (relexpr) -> (relexpr) -> Prop :=
+  Definition relexpr {A:Type}: Type := local_cstate * Σₕ * (program Σₕ A).
+  Definition rjoin {A:Type}: (@relexpr A) -> (relexpr) -> (relexpr) -> Prop :=
     fun '(σₗ1, σₕ1, cₕ1) '(σₗ2, σₕ2, cₕ2) '(σₗ3, σₕ3, cₕ3) =>
         join σₗ1.(st_mem) σₗ2.(st_mem) σₗ3.(st_mem) /\ 
         σₗ1.(lenv) = σₗ2.(lenv) /\ σₗ2.(lenv) = σₗ3.(lenv) /\
@@ -344,16 +287,16 @@ Section  SepRAssertion.
         σₕ1 = σₕ2 /\ σₕ2 = σₕ3 /\ 
         cₕ1 = cₕ2 /\ cₕ2 = cₕ3.
 
-  Definition ris_unit : (relexpr) -> Prop := fun '(σₗ1, σₕ1, cₕ1) => is_unit σₗ1.(st_mem).
+  Definition ris_unit {A:Type}: (@relexpr A) -> Prop := fun '(σₗ1, σₕ1, cₕ1) => is_unit σₗ1.(st_mem).
 
 
-  #[export] Instance reljoinm: @JoinM relexpr := {
+  #[export] Instance reljoinm {A:Type}: @JoinM (@relexpr A) := {
     join := rjoin;
     is_unit := ris_unit;
   }. 
-  Definition SepAhst (P : Σₕ -> Prop ): @relasrt local_cstate Σₕ (@denosem Σₕ):= fun '(σₗ, σₕ, cₕ) =>  P σₕ /\ is_unit σₗ.(st_mem).
+  Definition SepAhst {A:Type} (P : Σₕ -> Prop ): @relasrt local_cstate Σₕ (program Σₕ A):= fun '(σₗ, σₕ, cₕ) =>  P σₕ /\ is_unit σₗ.(st_mem).
 
-  Definition SepAspec (cₕ : @denosem Σₕ) : @relasrt local_cstate Σₕ (@denosem Σₕ):= fun '(σₗ, σₕ, c) =>  c = cₕ /\ is_unit σₗ.(st_mem).
+  Definition SepAspec {A:Type} (cₕ : (program Σₕ A)) : @relasrt local_cstate Σₕ (program Σₕ A):= fun '(σₗ, σₕ, c) =>  c = cₕ /\ is_unit σₗ.(st_mem).
 End SepRAssertion.
 
 Section  EncodeRules.
@@ -364,25 +307,26 @@ Section  EncodeRules.
 
 
 Local Open Scope sets_scope.
-Ltac destructs H:= rel_destruct local_cstate Σₕ Langstmts (@denosem Σₕ) H.
-Lemma encode_decomposed_sepcon: forall X (P: @asrt local_cstate) (P' : @asrt Σₕ) s,
+Ltac destructs A H:= rel_destruct local_cstate Σₕ Langstmts ((program Σₕ A)) H.
+
+Lemma encode_decomposed_sepcon {A:Type}: forall X (P: @asrt local_cstate) (P' : @asrt Σₕ) (s: (program Σₕ A)),
  [| ⌊ P ⌋ ** SepAhst P' ** SepAspec s|](X) --||--  !! (Exec P' s X) && P. 
 Proof.
   intros.
   intros σₗ;split.
   { unfold derivable1, sepcon, andp, coq_prop, encode_asrt, andp, Alst, SepAhst, SepAspec, Exec. simpl_hdefs. sets_unfold.
   intros.
-  destructs H.
+  destructs A H.
   simpl in *. 
   destruct x as ((? & ?) & ?). destruct x0 as ((? & ?) & ?).
   destruct x1 as ((? & ?) & ?). destruct x2 as ((? & ?) & ?).
   simpl in *.
-  destructs H4.
-  destructs H2.
+  destructs A H4.
+  destructs A H2.
   subst.
   destruct_st σₗ. destruct_st l. destruct_st l0. destruct_st l1. destruct_st l2.
-  cbn in *. subst. destructs H1. subst. 
-  destructs H0. subst.
+  cbn in *. subst. destructs A H1. subst. 
+  destructs A H0. subst.
   apply unit_spec in H1;auto.
   apply unit_spec in H0;auto.
   subst.
@@ -392,7 +336,7 @@ Proof.
 
   unfold derivable1, sepcon, andp, coq_prop, encode_asrt, andp, Alst, SepAhst, SepAspec, Exec. simpl_hdefs. sets_unfold.
   intros.
-  destructs H.
+  destructs A H.
   do 2 eexists.
   split;eauto.
   destruct_st σₗ.
@@ -422,14 +366,14 @@ Section  encrules.
 
   Local Open Scope sets_scope.
 
-  Ltac destructs H:= rel_destruct local_cstate Σₕ Langstmts (@denosem Σₕ) H.
+  Ltac destructs A H:= rel_destruct local_cstate Σₕ Langstmts ((program Σₕ A)) H.
 
   
 (**********************************************************************************)
 (*    trans reltriple into hoare triple                                           *)
 (**********************************************************************************)
 
-  Lemma  reltriple_triple_equiv1 : forall P Ps (s: @denosem Σₕ) c Q,
+  Lemma  reltriple_triple_equiv1 {A: Type}: forall P Ps (s: program Σₕ A) c Q,
     Δ ⩅ Γ ⊢ ⟨ ⌊ P ⌋ && ⌈ Ps ⌉ && [ s ]ₕ ⟩ c ⟨ Q ⟩ <->
     (forall X, (Δ ++ (| Γ |)) ⊢ {{!! Exec Ps s X && P}} c {{[| Q |](X)}}).
   Proof.
@@ -447,10 +391,10 @@ Section  encrules.
       cbv. auto.
   Qed.
 
-  Lemma  reltriple_triple_equiv {A: Type}: forall P Ps (s: @denosem Σₕ) c B Q Ps',
-    Δ ⩅ Γ ⊢ ⟨ ⌊ P ⌋ && ⌈ Ps ⌉ && [ s ]ₕ ⟩ c ⟨EX (a:A), !! (B a) && ⌊ Q a ⌋ && ⌈ Ps' a⌉ && [ skip ]ₕ ⟩ <->
-    (forall X : Σₕ -> Prop,
-    (Δ ++ (| Γ |)) ⊢ {{!! Exec Ps s X && P}} c {{EX a, !! Exec (Ps' a) skip X && !! (B a) && (Q a)}}).
+  Lemma  reltriple_triple_equiv {A R: Type}: forall P Ps (s: program Σₕ R) c B Q Ps',
+    Δ ⩅ Γ ⊢ ⟨ ⌊ P ⌋ && ⌈ Ps ⌉ && [ s ]ₕ ⟩ c ⟨EX (r: R) (a:A), !! (B a r) && ⌊ Q a r ⌋ && ⌈ Ps' a r⌉ && [ ret r ]ₕ ⟩ <->
+    (forall X : R -> Σₕ -> Prop,
+    (Δ ++ (| Γ |)) ⊢ {{!! Exec Ps s X && P}} c {{EX r a, !! Exec (Ps' a r) (ret r) X && !! (B a r) && (Q a r)}}).
   Proof.
     intros;split.
     - intros.
@@ -459,6 +403,9 @@ Section  encrules.
     eapply hoare_conseq;eauto.
     eapply (logic_equiv_derivable1_2 (encode_decomposed X P Ps s)).
     apply logic_equiv_derivable1_1.
+    eapply logic_equiv_trans.
+    apply logic_equiv_symm; apply (encode_exp_equiv _ _ ).
+    apply ex_logic_euiqv_elim_both;intros r.
     apply encode_normal_form.
     - intros. apply encoding_correctness.
       unfold valid_contextualrelT. intros.
@@ -466,51 +413,95 @@ Section  encrules.
       eapply hoare_conseq;eauto.
       apply (logic_equiv_derivable1_1 (encode_decomposed X P Ps s)).
       apply logic_equiv_derivable1_2.
+      eapply logic_equiv_trans.
+      apply logic_equiv_symm; apply (encode_exp_equiv _ _ ).
+      apply ex_logic_euiqv_elim_both;intros r.
       apply encode_normal_form.
   Qed.
 
-  Lemma high_focus_as_conseqpre cₗ (cₕ1 cₕ2: @denosem Σₕ) F P R Q:
-    forall X,
-    ⊢∃ {{P}} cₕ1 {{R}}  ->
-    (Δ ++ (| Γ |)) ⊢ {{!! Exec R cₕ2 X && F}} cₗ {{[|Q|](X)}} ->
-    (Δ ++ (| Γ |)) ⊢ {{!! Exec P (seq cₕ1 cₕ2) X && F}} cₗ {{[|Q|](X)}}.
+  Lemma high_focus_as_conseqpre {A B: Type} cₗ (cₕ1: program Σₕ A) (cₕ2: A -> program Σₕ B) F P R Q:
+    forall X a,
+    StateRelHoare.valid_angelic_triple P cₕ1 (fun r σ => r = a /\ R σ) -> 
+    (Δ ++ (| Γ |)) ⊢ {{!! Exec R (cₕ2 a) X && F}} cₗ {{[|Q|](X)}} ->
+    (Δ ++ (| Γ |)) ⊢ {{!! Exec P (bind cₕ1 cₕ2) X && F}} cₗ {{[|Q|](X)}}.
   Proof.
     intros.
     eapply hoare_conseq_pre;[ | eauto].
     apply derivable1_andp_mono;[ | reflexivity].
     apply coq_prop_imply.
-    eapply PracticalDenoExecLib.highstepseq_derive;eauto.
+    eapply highstepbind_derive.
+    eapply hs_eval_equiv_angelic_triple;auto.
   Qed.
 
-  Lemma comp_fc_as_conseq :forall 
-  P (cₗ: Langstmts) (cₕ: denosem) Q (Pₕ Qₕ: @asrt Σₕ),
-  ((forall X,  (Δ ++ (| Γ |)) ⊢ {{ [|↑ P && [cₕ ]ₕ|](X) }} cₗ {{ [|↑ Q && [skip ]ₕ|](X) }})) -> 
-  ⊢∀ {{ Pₕ }} cₕ {{ Qₕ }} ->
-   (Δ ++ (| Γ |)) ⊢ {{ P ⋈_π Pₕ }} cₗ {{ Q ⋈_π Qₕ }}.
+  Lemma comp_fc_as_conseq {A:Type}: forall 
+  P (cₗ: Langstmts) (cₕ: program Σₕ A) Q (Pₕ: @asrt Σₕ) Qₕ,
+  ((forall X,  (Δ ++ (| Γ |)) ⊢ {{ [|↑ P && [cₕ ]ₕ|](X) }} cₗ {{ [|EX a, ↑ Q a && [ret a ]ₕ|](X) }})) -> 
+  StateRelHoare.Hoare Pₕ cₕ Qₕ ->
+   (Δ ++ (| Γ |)) ⊢ {{ P ⋈_π Pₕ }} cₗ {{ EX a, (Q a) ⋈_π (Qₕ a) }}.
 Proof.
   intros * HRT HHT.
   eapply hoare_conseq_pre.  
   { apply (logic_equiv_derivable1_2 (comp_proj_equiv _ _ )). }
   eapply hoare_exists_intro; intros σₕ.
   eapply hoare_coqprop_preintro. intros HPH.
-  specialize (HRT (fun (x: Σₕ) => (nrm cₕ) σₕ x)).
+  specialize (HRT (fun r (x: Σₕ) => cₕ σₕ r x)).
   eapply hoare_conseq;eauto.
   - intros st1 ?.
     unfold encode_asrt, lift, basicasrt.andp, Aspec. simpl.
     do 2 eexists. split;[ | eauto].
-    specialize (HHT _ HPH)  as [? ?].
-    unfold weakestpre.
-    split;auto. 
+    unfold weakestpre. auto.
   - intros st1 HQ.
     unfold encode_asrt, lift, basicasrt.andp, Aspec in HQ.
-    destruct HQ as [σₕ' [cₕ' [? [? ?]]]]. subst. simpl_hdefs.
-    rewrite weakestpre_skip in H. simpl in H.
-    specialize (HHT _ HPH ) as [? ?].
-    specialize (H2 _ H).
+    destruct HQ as [σₕ' [cₕ' [? [? [? ?]]]]]. subst. simpl_hdefs.
+    unfold StateRelHoare.weakestpre in H. sets_unfold in H.
+    specialize (H x σₕ' (ltac:(unfold_monad;auto))). 
+    specialize (HHT _ _ _ HPH H).
+    exists x.
     do 2 eexists. cbv. split;eauto.
 Qed.
 
-End encrules.
 
-End RelJoinStateGlobalEnvHighNoCall.
+Lemma rh_hoare_vc_safeexec {A U V: Type}:forall Δ c (sₕ :  U -> program Σₕ A) P Ps Q Qs B1 B2 Pₕ Qₕ u,
+  (Hoare (Pₕ) (sₕ u) (Qₕ)) ->
+  (forall X,  Δ ⊢ {{EX (u: U), !! Exec (Ps u) (sₕ u) X && !! (B1 u) && (P u)}} c 
+      {{EX (r: A) (v: V), !! Exec (Qs v r) (ret r) X && !! (B2 v r) && (Q v r) }}) ->
+  (Δ  ⊢ {{ !! (exists s, Ps u s /\ Pₕ s) && !! (B1 u) && (P u) }} c 
+        {{EX r v, !! (exists s, Qs v r s /\ Qₕ r s) && !! (B2 v r) && (Q v r) }}).
+Proof.
+  intros * HHT HRT.
+  eapply hoare_conseq_pre.
+  { eapply logic_equiv_derivable1_1. apply logic_equiv_andp_assoc.  }
+  eapply hoare_coqprop_preintro;intros [σₕ [? HPH]].
+  specialize (HRT (fun r (x: Σₕ) => (sₕ u) σₕ r x)).
+  eapply hoare_conseq;eauto.
+  - eapply shallow_exp_right with (x:= u).
+    eapply derivable1_andp_mono;[ | reflexivity].
+    eapply logic_equiv_derivable1_2.
+    apply prop_andp_elim_equiv.
+    unfold Exec. simpl_hdefs. sets_unfold. eexists. 
+    split;[ eauto | ].
+    unfold weakestpre. auto.
+  - apply shallow_exp_left; intros a.
+    apply shallow_exp_left; intros v.
+    eapply shallow_exp_right with (x:= a).
+    eapply shallow_exp_right with (x:= v).
+    eapply derivable1_andp_mono;[ | reflexivity].
+    eapply derivable1_andp_mono;[ | reflexivity].
+    apply coq_prop_imply.
+    unfold Exec. simpl_hdefs. sets_unfold. unfold weakestpre. 
+    intros [σₕ' [? ?]].
+    specialize (H1 a σₕ' (ltac:(unfold_monad;auto))).
+    specialize (HHT _ _ _ HPH H1).
+    eexists.  split;eauto.
+  Qed.
+
+
+  End encrules. 
+End RelImpAbsMonad.
+
+
+
+
+
+
 
