monadlib/StateRelMonad/safeexec_lib.v
@@ -5,16 +5,20 @@ Require Import Coq.Classes.Morphisms.
 Require Import Coq.Lists.List.
 From SetsClass Require Import SetsClass.
 From MonadLib.StateRelMonad Require Import StateRelBasic StateRelHoare.
+From EncRelSeq.Basics Require Import basictacs basicasrt.
+From EncRelSeq.Basics Require Export encdefs.
+
+Import SetsNotation.
+Local Open Scope sets_scope.
+Local Open Scope asrt_scope.
+
+#[export] Instance staterelmonad_highlevel_defs {Σ A: Type} : highlevel_defs Σ (program Σ A) (A -> Σ -> Prop) := {|
+  highlevel_wlp := @weakestpre Σ A
+|}.
 
 Import Monad SetsNotation MonadNotation.
 Local Open Scope sets.
 Local Open Scope monad.
-
-Definition safe {Σ: Type} {A: Type} (σ : Σ) (c:  program Σ A) (X : A -> Σ -> Prop) := 
-    forall r σ', c σ r σ' -> (r, σ') ∈ X.  
-
-Definition safeExec {Σ: Type} {A: Type} (P: Σ -> Prop) (c: program Σ A) (X: A -> Σ -> Prop) :=
-  exists σₕ, P σₕ /\ safe σₕ c X.
 
 Definition result_state {Σ A: Type} (P: Σ -> Prop) (c: program Σ A): A -> Σ -> Prop :=
   fun a s1 => exists s0, P s0 /\ c s0 a s1. 
@@ -27,49 +31,37 @@ Notation " P '-@' s '-⥅' P' '♯' a " := (hs_eval s P P' a) (at level 70, no a
 
 Notation " P '-@' s '-→' P' " := (exists a,  hs_eval s P P' a) (at level 70, no associativity).
 
-(**********************************************************************************)
-(*    safe exec  rules                                                            *)
-(**********************************************************************************)
-Ltac splits :=
-  match goal with 
-  | |- _ /\ _ => split;splits
-  | |- _ => idtac end.
-
-Local Ltac my_destruct Σ H :=
-  match type of H with
-  | exists (_ : ?A), _ =>  
-              match A with 
-              | Σ => let σ := fresh "σₕ" in destruct H as [σ H];my_destruct Σ H
-              | program Σ ?A => let c := fresh "c" in destruct H as [c H];my_destruct Σ H
-              | _ => destruct H as [? H];my_destruct Σ H
-              end
-  | _ /\ _ => let H0 := fresh "H" in 
-              destruct H as [H H0];
-              my_destruct Σ H;
-              my_destruct Σ H0
-  | _ \/ _ => destruct H as [H | H];
-              my_destruct Σ H
-  | _ => (discriminate || contradiction  || idtac)
-  end.
-
 Section  safeexec_rules.
   Context {Σ: Type}.
 
   Definition asrt : Type :=  Σ -> Prop.
 
-  Ltac destructs H := my_destruct Σ H.
+  Ltac destructs H := st_destruct Σ H.
   Lemma ret_eq : forall {A : Type} (s: Σ) s0 (a a0: A),
     (ret a) s a0 s0 <-> s = s0 /\ a0 = a.
   Proof.
     unfold_monad; tauto.
   Qed.
 
-  Lemma highstependret_derive : forall  {A : Type} (c1: program Σ A)  (P  : Σ -> Prop) a P',
-  P -@ c1 -⥅ (P' a) ♯ a ->
-  (forall X, safeExec P (c1) X ->  safeExec (P' a) (ret a) X).
+  Lemma hs_eval_equiv_angelic_triple: forall {A : Type} (c1: program Σ A)  (P  : Σ -> Prop) a Q, 
+    P -@ c1 -⥅ Q ♯ a <->
+    valid_angelic_triple P c1 (fun r σ => r = a /\ Q σ).
   Proof.
     intros.
-    unfold hs_eval, safeExec, safe in *.
+    unfold hs_eval, valid_angelic_triple. unfold_monad.
+    split;intros.
+    - specialize (H _ H0) as (? & ? & ?).
+      eexists. splits;eauto.
+    - specialize (H _ H0) as (? & ? & ? & ? & ?). subst.
+      eexists. splits;eauto.
+  Qed. 
+
+  Lemma highstependret_derive : forall  {A : Type} (c1: program Σ A)  (P  : Σ -> Prop) a P',
+  P -@ c1 -⥅ (P' a) ♯ a ->
+  (forall X, Exec P (c1) X ->  Exec (P' a) (ret a) X).
+  Proof.
+    intros.
+    unfold hs_eval, Exec in *; simpl in *. unfold weakestpre in *. 
     destructs H0. 
     simpl in *.
     specialize (H _ H0) as [σₕ' [? ?]].
@@ -84,7 +76,7 @@ Section  safeexec_rules.
 
   Lemma highstepend_derive : forall  (c1: program Σ unit)  (P  : Σ -> Prop) P',
   P -@ c1 -→ P' ->
-  (forall X, safeExec P (c1) X ->  safeExec P' (ret tt) X).
+  (forall X, Exec P (c1) X ->  Exec P' (ret tt) X).
   Proof.
     intros.
     destruct H.
@@ -95,10 +87,10 @@ Section  safeexec_rules.
 
   Lemma highstepbind_derive : forall {A B: Type} (c1: program Σ A) (c2: A -> program Σ B) (P  : Σ -> Prop) a P',
   P -@ c1 -⥅ (P') ♯ a ->
-  (forall X, safeExec P (x <- c1;; c2 x) X ->  safeExec (P') (c2 a) X).
+  (forall X, Exec P (x <- c1;; c2 x) X ->  Exec (P') (c2 a) X).
   Proof.
     intros.
-    unfold hs_eval, safeExec, safe in *.
+    unfold hs_eval, Exec in *; simpl in *. unfold weakestpre in *. 
     destructs H0. 
     simpl in *.
     specialize (H _ H0) as [σₕ' [? ?]].
@@ -112,7 +104,7 @@ Section  safeexec_rules.
 
   Lemma highstepseq_derive : forall  {A B: Type} (c1: program Σ A) (c2:  program Σ B) (P P': Σ -> Prop),
     P -@ c1 -→ P'  ->
-    (forall X, safeExec P (c1 ;; c2) X ->  safeExec P' c2 X).
+    (forall X, Exec P (c1 ;; c2) X ->  Exec P' c2 X).
   Proof.
     intros.
     destruct H.
@@ -202,10 +194,10 @@ Section  safeexec_rules.
     eauto.
   Qed.
 
-  Lemma safeExec_ex : forall {A B: Type} (P: A -> Σ -> Prop) (c:  program Σ B) X,
-  (exists a, safeExec (P a) (c) X) <->  safeExec (fun σ => exists a, P a σ) (c) X.
+  Lemma Exec_ex : forall {A B: Type} (P: A -> Σ -> Prop) (c:  program Σ B) X,
+  (exists a, Exec (P a) (c) X) <->  Exec (fun σ => exists a, P a σ) (c) X.
   Proof.
-    unfold safeExec;intros;split;intros.
+    unfold Exec;simpl;unfold weakestpre;intros;split;intros.
     - destruct H as (? & ? & ? & ?).
       eexists.
       split;eauto.
@@ -214,12 +206,11 @@ Section  safeexec_rules.
       split;eauto.
   Qed. 
 
-
-  Lemma safeExec_prorefine: forall {A : Type} (c1 c2: program Σ A)  (P  : Σ -> Prop) X,
+  Lemma Exec_prorefine: forall {A : Type} (c1 c2: program Σ A)  (P  : Σ -> Prop) X,
   c2 ⊆ c1 ->
-  safeExec P c1 X -> safeExec P c2 X.
+  Exec P c1 X -> Exec P c2 X.
   Proof.
-    unfold safeExec. intros.
+    unfold Exec;simpl;unfold weakestpre; intros.
     destructs H0.
     eexists.
     split;eauto.
@@ -229,23 +220,23 @@ Section  safeexec_rules.
     eapply H1;eauto.
   Qed.
 
-  Lemma safeExec_X_subset {A: Type} (c: program Σ A) (P: Σ -> Prop) X1 X2:
+  Lemma Exec_X_subset {A: Type} (c: program Σ A) (P: Σ -> Prop) X1 X2:
     X1 ⊆ X2 ->
-    safeExec P c X1 ->
-    safeExec P c X2.
+    Exec P c X1 ->
+    Exec P c X2.
   Proof.
-    unfold safeExec, safe; intros Hx [s [H1 H2]].
+    unfold Exec;simpl;unfold weakestpre; intros Hx [s [H1 H2]].
     exists s; split; auto.
     intros a s' H3.
-    rewrite <- Hx.
+    apply Hx.
     apply H2; auto.
   Qed.
 
-  Lemma safeExec_proequiv: forall {A : Type} (c1 c2: program Σ A)  (P  : Σ -> Prop) X,
-  c1 == c2 ->
-  safeExec P c1 X -> safeExec P c2 X.
+  Lemma Exec_proequiv: forall {A : Type} (c1 c2: program Σ A)  (P  : Σ -> Prop) X,
+    c1 == c2 ->
+    Exec P c1 X -> Exec P c2 X.
   Proof.
-    unfold safeExec. intros.
+    unfold Exec;simpl;unfold weakestpre; intros.
     destructs H0.
     eexists.
     split;eauto.
@@ -269,18 +260,18 @@ Section  safeexec_rules.
     eapply H;eauto.
   Qed.
 
-  Lemma safeExec_bind : forall {A B: Type} (c1: program Σ A) (c2: A -> program Σ B) (P : Σ -> Prop) ,
-    forall X, safeExec P (x <- c1 ;; c2 x) X ->
-    exists X', safeExec P c1 X' /\
-    (forall P' a, safeExec P'  (ret a) X' -> 
-              safeExec P' (c2 a) X).
+  Lemma Exec_bind : forall {A B: Type} (c1: program Σ A) (c2: A -> program Σ B) (P : Σ -> Prop) ,
+    forall X, Exec P (x <- c1 ;; c2 x) X ->
+    exists X', Exec P c1 X' /\
+    (forall P' a, Exec P'  (ret a) X' -> 
+              Exec P' (c2 a) X).
   Proof.
     intros.
-    unfold safeExec in H.
+    unfold Exec in H. simpl_hdefs.
     destructs H.
-    unfold safe in H0.
-    exists (fun (r : A) (x : Σ) => c1 σₕ r x).
-    unfold safeExec.
+    unfold weakestpre in H0.
+    exists (fun (r : A) (x : Σ) => c1 st r x).
+    unfold Exec. simpl_hdefs;unfold weakestpre. sets_unfold.
     splits;eauto.
     { eexists.
       split;eauto.
@@ -291,8 +282,8 @@ Section  safeexec_rules.
     destructs H1.
     eexists.
     split;eauto.
-    unfold safe in H2; unfold_monad in H2.
-    specialize (H2 a σₕ0  (ltac:(auto))).
+    unfold_monad in H2.
+    specialize (H2 a st0 (ltac:(auto))).
     unfold safe.
     intros.
     eapply H0.
@@ -302,12 +293,12 @@ Section  safeexec_rules.
     split;eauto.
   Qed. 
 
-  Lemma safeExec_bind_high {A B: Type}: forall a (Q: A -> Σ -> Prop) (P : Σ -> Prop) (c1: program Σ A) (c2: A -> program Σ B) X,
-    safeExec P (x <- c1;; c2 x) X ->
+  Lemma Exec_bind_high {A B: Type}: forall a (Q: A -> Σ -> Prop) (P : Σ -> Prop) (c1: program Σ A) (c2: A -> program Σ B) X,
+    Exec P (x <- c1;; c2 x) X ->
     (forall s1, P s1 -> exists s2, c1 s1 a s2 /\ Q a s2) ->
-    safeExec (Q a) (c2 a) X.
+    Exec (Q a) (c2 a) X.
   Proof.
-    unfold safeExec, safe; unfold_monad; sets_unfold; intros.
+    unfold Exec;simpl_hdefs;unfold weakestpre; unfold_monad; sets_unfold; intros.
     destruct H as [s [HP Hs]].
     specialize (H0 s HP); destruct H0 as [s1 [Hc1 Qs2]].
     exists s1; split; auto.
@@ -316,12 +307,12 @@ Section  safeexec_rules.
     exists a, s1; tauto.
   Qed.
 
-  Lemma safeExec_bind_unit {B: Type}: forall (Q: Σ -> Prop) (P : Σ -> Prop) (c1: program Σ unit) (c2:program Σ B) X,
-    safeExec P (c1;; c2) X ->
+  Lemma Exec_bind_unit {B: Type}: forall (Q: Σ -> Prop) (P : Σ -> Prop) (c1: program Σ unit) (c2:program Σ B) X,
+    Exec P (c1;; c2) X ->
     (forall s1, P s1 -> exists s2, c1 s1 tt s2 /\ Q s2) ->
-    safeExec Q c2 X.
+    Exec Q c2 X.
   Proof.
-    unfold safeExec, safe; unfold_monad; sets_unfold; intros.
+    unfold Exec;simpl_hdefs;unfold weakestpre; unfold_monad; sets_unfold; intros.
     destruct H as [s [HP Hs]].
     specialize (H0 s HP); destruct H0 as [s1 [Hc1 Qs2]].
     exists s1; split; auto.
@@ -330,69 +321,69 @@ Section  safeexec_rules.
     exists tt, s1; tauto.
   Qed.
 
-  Lemma safeExec_conseq: forall {A: Type} (P' P: Σ -> Prop) (c: program Σ A)  X,
-    safeExec P c X ->
+  Lemma Exec_conseq: forall {A: Type} (P' P: Σ -> Prop) (c: program Σ A)  X,
+    Exec P c X ->
     (forall s, P s -> P' s) ->
-    safeExec P' c X.
+    Exec P' c X.
   Proof.
-    unfold safeExec, safe; intros.
+    unfold Exec;simpl_hdefs;unfold weakestpre;sets_unfold; intros.
     destruct H as [hs [Ps Hc]].
     exists hs; split; auto.
   Qed.
   
-  (* Lemma safeExec_bind'  : forall {A B: Type} (c1: program Σ A) (c2: A -> program Σ B) (P : Σ -> Prop) P',
-    (forall X, safeExec P c1 X -> exists a, safeExec (P')  (ret a) X) ->
-    (forall X, safeExec P (x <- c1 ;; c2 x) X -> exists a, safeExec (P') (c2 a) X). *)
+  (* Lemma Exec_bind'  : forall {A B: Type} (c1: program Σ A) (c2: A -> program Σ B) (P : Σ -> Prop) P',
+    (forall X, Exec P c1 X -> exists a, Exec (P')  (ret a) X) ->
+    (forall X, Exec P (x <- c1 ;; c2 x) X -> exists a, Exec (P') (c2 a) X). *)
 
-  Lemma safeExec_choice_left: forall {A: Type} (c1 c2: program Σ A) P X,
-    safeExec P (choice c1 c2) X ->
-    safeExec P c1 X.
+  Lemma Exec_choice_left: forall {A: Type} (c1 c2: program Σ A) P X,
+    Exec P (choice c1 c2) X ->
+    Exec P c1 X.
   Proof.
-    unfold safeExec, choice, safe.
+    unfold Exec, choice;simpl_hdefs;unfold weakestpre;sets_unfold.
     intros.
     destruct H as [σ [? ?]].
     exists σ.
-    split; [tauto |].
+    split; [tauto | ].
     intros.
     specialize (H0 r σ' ltac:(left; tauto)).
     tauto.
   Qed.
 
-  Lemma safeExec_choice_right: forall {A: Type} (c1 c2: program Σ A) P X,
-    safeExec P (choice c1 c2) X ->
-    safeExec P c2 X.
+  Lemma Exec_choice_right: forall {A: Type} (c1 c2: program Σ A) P X,
+    Exec P (choice c1 c2) X ->
+    Exec P c2 X.
   Proof.
-    unfold safeExec, choice, safe.
+    unfold Exec, choice;simpl_hdefs;unfold weakestpre;sets_unfold.
     intros.
     destruct H as [σ [? ?]].
     exists σ.
-    split; [tauto |].
+    split; [tauto | ].
     intros.
     specialize (H0 r σ' ltac:(right; tauto)).
     tauto.
   Qed.
 
-  Lemma safeExec_test_bind: forall {A: Type} (Q: Prop) (c: program Σ A) P X,
+  Lemma Exec_test_bind: forall {A: Type} (Q: Prop) (c: program Σ A) P X,
     Q ->
-    safeExec P (assume!! Q ;; c) X ->
-    safeExec P c X.
+    Exec P (assume!! Q ;; c) X ->
+    Exec P c X.
   Proof.
     intros.
-    eapply (safeExec_bind_high tt (fun _ => P)) in H0; auto.
+    eapply (Exec_bind_high tt (fun _ => P)) in H0; auto.
     unfold test'; intros.
     exists s1; tauto.
   Qed.
 
-  Lemma safeExec_testst_bind: forall {A: Type} (Q: Σ -> Prop) (c: program Σ A) (P: Σ -> Prop) X,
+  Lemma Exec_testst_bind: forall {A: Type} (Q: Σ -> Prop) (c: program Σ A) (P: Σ -> Prop) X,
     (forall st, P st -> Q st) ->
-    safeExec P (assume Q;; c) X ->
-    safeExec P c X.
+    Exec P (assume Q;; c) X ->
+    Exec P c X.
   Proof.
-    unfold safeExec, test, safe, seq, bind.
+    unfold Exec, test, bind;simpl_hdefs;unfold weakestpre;sets_unfold.
     intros.
     destruct H0 as [σ [? ?]].
     exists σ.
-    split; [tauto |].
+    split; [tauto | ].
     intros.
     apply (H1 r σ').
     exists tt, σ.
@@ -400,15 +391,15 @@ Section  safeexec_rules.
     splits;auto.
   Qed.
 
-  Lemma safeExec_any_bind: forall {A: Type} (Q: Type) (c: Q -> program Σ A) (P: Σ -> Prop) X a,
-    safeExec P (a <- any Q;; c a) X ->
-    safeExec P (c a) X.
+  Lemma Exec_any_bind: forall {A: Type} (Q: Type) (c: Q -> program Σ A) (P: Σ -> Prop) X a,
+    Exec P (a <- any Q;; c a) X ->
+    Exec P (c a) X.
   Proof.
-    unfold safeExec, any, safe, seq, bind.
+    unfold Exec, any, bind;simpl_hdefs;unfold weakestpre;sets_unfold.
     intros.
     destruct H as [σ [? ?]].
     exists σ.
-    split; [tauto |].
+    split; [tauto | ].
     intros.
     apply (H0 r σ').
     exists a, σ.
@@ -416,34 +407,34 @@ Section  safeexec_rules.
     splits;auto.
   Qed.
 
-  Lemma safeExec_get_bind {A B: Type} (a: A) (Pa: Σ -> A -> Prop) (P: Σ -> Prop) (c: A -> program Σ B) X:
+  Lemma Exec_get_bind {A B: Type} (a: A) (Pa: Σ -> A -> Prop) (P: Σ -> Prop) (c: A -> program Σ B) X:
     (forall s, P s -> Pa s a) ->
-    safeExec P (a0 <- get Pa;; c a0) X ->
-    safeExec P (c a) X.
+    Exec P (a0 <- get Pa;; c a0) X ->
+    Exec P (c a) X.
   Proof.
     intros.
-    apply ( safeExec_bind_high  a (fun _ => P)) in H0; auto.
+    apply ( Exec_bind_high  a (fun _ => P)) in H0; auto.
     intros; unfold get.
     exists s1; split; auto.
   Qed.
 
-  Lemma safeExec_update'_bind {B: Type} (f: Σ -> Σ) (P: Σ -> Prop) (c:program Σ B) X:
-    safeExec P (update' f;; c) X ->
-    safeExec (fun s => exists s0, s = f s0 /\ P s0) c X.
+  Lemma Exec_update'_bind {B: Type} (f: Σ -> Σ) (P: Σ -> Prop) (c:program Σ B) X:
+    Exec P (update' f;; c) X ->
+    Exec (fun s => exists s0, s = f s0 /\ P s0) c X.
   Proof.
     intros.
-    eapply safeExec_bind_unit; eauto.
+    eapply Exec_bind_unit; eauto.
     unfold update', update; intros.
     exists (f s1).
     split; auto.
     exists s1; tauto.
   Qed.
 
-  Lemma safeExec_bind_rightsubst : forall {A B: Type} (c1: program Σ A) (c2 c2': A -> program Σ B) (P : Σ -> Prop) X X',
+  Lemma Exec_bind_rightsubst : forall {A B: Type} (c1: program Σ A) (c2 c2': A -> program Σ B) (P : Σ -> Prop) X X',
     (forall σ a, safe σ (c2 a) X -> safe σ (c2' a) X') ->
-    (safeExec P (x <- c1 ;; c2 x) X -> safeExec P (x <- c1 ;; c2' x) X').
+    (Exec P (x <- c1 ;; c2 x) X -> Exec P (x <- c1 ;; c2' x) X').
   Proof.
-    unfold safeExec,safe.
+    unfold Exec, safe;simpl_hdefs;unfold weakestpre;sets_unfold.
     unfold_monad.
     intros.
     destructs H0.
@@ -457,42 +448,43 @@ Section  safeexec_rules.
     eapply H; eauto.
   Qed.
 
-  Lemma safeExec_subst : forall {A: Type} (c1 c1': program Σ A)  (P : Σ -> Prop) X X',
+  Lemma Exec_subst : forall {A: Type} (c1 c1': program Σ A)  (P : Σ -> Prop) X X',
     (forall σ, safe σ c1 X -> safe σ c1' X') ->
-    (safeExec P (c1) X -> safeExec P (c1') X').
+    (Exec P (c1) X -> Exec P (c1') X').
   Proof.
-    unfold safeExec,safe.
+    unfold Exec, safe.
     intros.
     destructs H0.
     eexists.
     split;eauto.
   Qed.
 
-  Lemma safeExec_monad_Atrue_finnal: forall  {A: Type} (m: program unit A) ,
-    safeExec ATrue m (fun r x => m tt r x).
+  Lemma Exec_monad_Atrue_finnal: forall  {A: Type} (m: program unit A) ,
+    Exec ATrue m (fun r x => m tt r x).
   Proof.
     intros.
-    unfold safeExec, ATrue, safe.
+    unfold Exec, ATrue;simpl_hdefs;unfold weakestpre;sets_unfold.
     exists tt.
     splits;auto.
   Qed.
 
-  Lemma safeExec_ret_Atrue_finnal: forall  {A: Type}  (m: program Σ A) (l : A) (σ: Σ) ,
-    safeExec ATrue (ret l) (fun r x => m σ r x) ->
+  Lemma Exec_ret_Atrue_finnal: forall  {A: Type}  (m: program Σ A) (l : A) (σ: Σ) ,
+    Exec ATrue (ret l) (fun r x => m σ r x) ->
     exists σ', m σ l σ'.
   Proof.
-    unfold safeExec,safe; unfold_monad.
+    unfold Exec, ATrue;simpl_hdefs;unfold weakestpre;sets_unfold.
     intros.
     destructs H.
-    specialize (H0 l σₕ (ltac:(auto))).
-    exists σₕ.
+    specialize (H0 l st (ltac:(unfold_monad;auto))).
+    exists st.
     auto.
   Qed.
 
-  Lemma safeExec_choice_l {A: Type}:
+  Lemma Exec_choice_l {A: Type}:
     forall (c0 c1: program Σ A) X (s: Σ -> Prop),
-      safeExec s (choice c0 c1) X -> safeExec s c0 X.
+      Exec s (choice c0 c1) X -> Exec s c0 X.
   Proof.
+    unfold Exec;simpl_hdefs;unfold weakestpre.
     intros.
     destruct H as [? [? ?]].
     unfold safe in *.
@@ -506,10 +498,11 @@ Section  safeexec_rules.
   Qed.
   
   (* same as choice_l *)
-  Lemma safeExec_choice_r {A: Type}:
+  Lemma Exec_choice_r {A: Type}:
     forall (c0 c1: program Σ A) X (s: Σ -> Prop),
-      safeExec s (choice c0 c1) X -> safeExec s c1 X.
+      Exec s (choice c0 c1) X -> Exec s c1 X.
   Proof.
+    unfold Exec;simpl_hdefs;unfold weakestpre.
     intros.
     destruct H as [? [? ?]].
     unfold safe in *.
@@ -522,24 +515,25 @@ Section  safeexec_rules.
     tauto.
   Qed.
 
-  Lemma safeExec_test' {A: Type}:
+  Lemma Exec_test' {A: Type}:
     forall (s: Σ -> Prop) (P: Prop) (c: program Σ A) X,
       P ->
-      safeExec s (test' P;; c) X ->
-      safeExec s c X.
+      Exec s (test' P;; c) X ->
+      Exec s c X.
   Proof.
-    intros; unfold safeExec in *.
+    unfold Exec;simpl_hdefs;unfold weakestpre.
+    intros.
     destructs H0.
-    exists σₕ.
+    exists st.
     split; auto.
-    unfold safe in *.
+    sets_unfold.
     intros.
     specialize (H1 r σ').
     unfold test' in H1; simpl in H1.
     unfold_monad in H1.
     sets_unfold in H1.
     apply H1.
-    exists tt; exists σₕ; tauto.
+    exists tt; exists st; tauto.
   Qed.
 
   Lemma hseval_stateless_ret: forall  {A: Type}  (m: program unit A) (a : A),
@@ -552,63 +546,63 @@ Section  safeexec_rules.
     easy.
   Qed.
   
-  Lemma safeExec_ret {A: Type} a (P: Σ -> Prop) (X: A -> Σ -> Prop):
-    safeExec P (ret a) X ->
+  Lemma Exec_ret {A: Type} a (P: Σ -> Prop) (X: A -> Σ -> Prop):
+    Exec P (ret a) X ->
     exists s, P s /\ (a, s) ∈ X.
   Proof.
-    unfold safeExec, safe; unfold_monad.
+    unfold Exec;simpl_hdefs;unfold weakestpre. unfold_monad.
     intros [s [? ?]].
     specialize (H0 a s).
     exists s; tauto.
   Qed.
 
-  Lemma safeExec_ret_tt (P: Σ -> Prop) (X: Σ -> Prop):
-    safeExec P (ret tt) (fun _ => X) ->
+  Lemma Exec_ret_tt (P: Σ -> Prop) (X: Σ -> Prop):
+    Exec P (ret tt) (fun _ => X) ->
     exists s, P s /\  X s.
   Proof.
-    intros; apply safeExec_ret in H.
+    intros; apply Exec_ret in H.
     sets_unfold in H; auto.
   Qed.
 
 End  safeexec_rules.
 
-#[export] Instance safeExec_programrefine_impl_Proper
+#[export] Instance Exec_programrefine_impl_Proper
   {Σ: Type} {A: Type} (P: Σ -> Prop):
-  Proper (Sets.included ==> eq ==> (Basics.flip Basics.impl)) (@safeExec Σ A P).
+  Proper (Sets.included ==> eq ==> (Basics.flip Basics.impl)) (@Exec Σ (program Σ A) _ _ P).
 Proof.
   unfold Proper, respectful.
   intros. subst y0.
   hnf.
-  apply safeExec_prorefine;eauto.
+  apply Exec_prorefine;eauto.
 Qed.
 
-#[export] Instance safeExec_X_subset_impl_Proper
+#[export] Instance Exec_X_subset_impl_Proper
   {Σ: Type} {A: Type} (P: Σ -> Prop):
-  Proper (eq ==> Sets.included ==> Basics.impl) (@safeExec Σ A P).
+  Proper (eq ==> Sets.included ==> Basics.impl) (@Exec Σ (program Σ A) _ _ P).
 Proof.
   unfold Proper, respectful.
   intros; subst.
-  hnf; apply safeExec_X_subset; auto.
+  hnf; apply Exec_X_subset; auto.
 Qed.
 
-#[export] Instance safeExec_programequiv_iff_Proper
+#[export] Instance Exec_programequiv_iff_Proper
   {Σ: Type} {A: Type} (P: Σ -> Prop):
-  Proper (Sets.equiv ==> eq ==>  iff) (@safeExec Σ A P).
+  Proper (Sets.equiv ==> eq ==>  iff) (@Exec Σ (program Σ A) _ _ P).
 Proof.
   unfold Proper, respectful.
   intros. subst y0. split. 
-  apply safeExec_proequiv. auto.
-  apply safeExec_proequiv. symmetry. auto.
+  apply Exec_proequiv. auto.
+  apply Exec_proequiv. symmetry. auto.
 Qed.
 
-#[export] Instance safeExec_programequiv_iff_Proper'
+#[export] Instance Exec_programequiv_iff_Proper'
   {Σ: Type} {A: Type} (P: Σ -> Prop):
-  Proper (Sets.equiv ==> eq ==>  iff) (@safeExec Σ A P).
+  Proper (Sets.equiv ==> eq ==>  iff) (@Exec Σ (program Σ A) _ _ P).
 Proof.
   unfold Proper, respectful.
   intros. subst y0. split. 
-  apply safeExec_proequiv. auto.
-  apply safeExec_proequiv. symmetry. auto.
+  apply Exec_proequiv. auto.
+  apply Exec_proequiv. symmetry. auto.
 Qed.
 
 #[export] Instance hseval_programequiv_Proper
@@ -643,7 +637,7 @@ Arguments program_para_equiv {Σ} {A B}%type_scope [f1] [f2].
 
 Ltac __prove_by_one_abs_step x :=
   match goal with
-  | H: safeExec ?P1 (bind ?c11 ?c12) ?X |- safeExec ?P2 ?c2 ?X =>
+  | H: Exec ?P1 (bind ?c11 ?c12) ?X |- Exec ?P2 ?c2 ?X =>
       unify (c12 x) c2; 
       refine (highstepbind_derive _ _ _ x P2 _ X H);
       clear H
@@ -676,29 +670,29 @@ Ltac abs_ret_step :=
 
 Ltac safe_step H := prog_nf in H;
   match type of H with
-  | safeExec _ ((test' _ ) ;; _) _ => apply safeExec_test' in H; [try safe_step H | auto]
+  | Exec _ ((test' _ ) ;; _) _ => apply Exec_test' in H; [try safe_step H | auto]
   end.
 
 Ltac safe_choice_l H :=
-  prog_nf in H;apply safeExec_choice_l in H; try safe_step H.
+  prog_nf in H;apply Exec_choice_l in H; try safe_step H.
 
 Ltac safe_choice_r H :=
-  prog_nf in H;apply safeExec_choice_r in H; try safe_step H.
+  prog_nf in H;apply Exec_choice_r in H; try safe_step H.
 
 Ltac safe_equiv :=
-  eapply safeExec_proequiv; eauto.  
+  eapply Exec_proequiv; eauto.  
 
 
 Section  safeexec_Hoare_composition_rules.
   
   Context {Σ: Type}.
 
-  Ltac destructs H := my_destruct Σ H.
-  Lemma safeExec_result_state {A: Type} (P: Σ -> Prop) (c: program Σ A):
+  Ltac destructs H := st_destruct Σ H.
+  Lemma Exec_result_state {A: Type} (P: Σ -> Prop) (c: program Σ A):
     (exists s, P s) ->
-    safeExec P c (result_state P c).
+    Exec P c (result_state P c).
   Proof.
-    unfold safeExec, result_state, safe.
+    unfold Exec, result_state, safe.
     intros [s HP].
     exists s; split; auto.
     sets_unfold; intros a s' ?.
@@ -717,15 +711,15 @@ Section  safeexec_Hoare_composition_rules.
   Lemma Hoare_safeexec_compose {A: Type} (P1 : Σ -> Prop) (c: program Σ A) (Q: A -> Σ -> Prop):
     Hoare P1 c Q ->
     forall (P2: Σ -> Prop) (a: A) (σ : Σ),
-    safeExec P2 (return a) (c σ) -> 
+    Exec P2 (return a) (c σ) -> 
     σ ∈ P1 ->
     (exists σ', Q a σ' /\ P2 σ').
   Proof.
-    unfold Hoare, safeExec, safe.
+    unfold Hoare, Exec;simpl_hdefs;unfold weakestpre.
     intros. 
     destructs H0.
     sets_unfold.
-    specialize (H2 a σₕ (ltac:(unfold_monad;auto))).
+    specialize (H2 a st (ltac:(unfold_monad;auto))).
     specialize (H σ _ _ H1 H2).
     eexists. eauto.
   Qed.
