EncRelSeq/MonadsAsHigh/AbsMonad/relhoarelogic.v
@@ -1,0 +1,184 @@
+Require Import Coq.Classes.RelationClasses.
+From SetsClass Require Import SetsClass.
+Require Import MonadLib.MonadLib.
+Import StateRelMonad.
+From EncRelSeq.Basics Require Import basicasrt relasrt.
+From EncRelSeq Require Export semantics errsem.
+
+Local Open Scope sets_scope.
+
+Module ConfigReineStatreRelMonad.
+
+(* Configuration Refinement *)
+Definition config_refinement {Σ A: Type} (g1 g2: (Σ * program Σ A)%type ) : Prop :=
+  let '(σ1, c1) := g1 in
+  let '(σ2, c2) := g2 in
+  (forall r σ₃, c2 σ2 r σ₃ -> c1 σ1 r σ₃).
+
+Arguments config_refinement: simpl never.
+Notation " g1 '↪' g2 " := (config_refinement g1 g2) (at level 28, left associativity).
+
+#[export] Instance configrefine_reflexivity {Σ A: Type}: Reflexive (@config_refinement Σ A).
+Proof.
+  hnf. unfold config_refinement. intros. intuition eauto. Qed. 
+#[export] Instance configrefine_refinement_transivity {Σ A: Type}: Transitive (@config_refinement Σ A).
+Proof.
+  hnf. unfold config_refinement. intros [? ?] [? ?] [? ?]. intuition eauto. Qed. 
+
+
+Section config_refinement_rules.
+  Context {Σ A B: Type}.
+
+  Import MonadNotation.
+  Local Open Scope monad.
+
+  Lemma config_refinement_ret : forall (c: program Σ A) (σ1 σ2: Σ) a,
+    c σ1 a σ2 <->
+    ( σ1, c ) ↪ ( σ2, ret a).
+  Proof.
+    intros; unfold config_refinement; simpl; unfold_monad; sets_unfold; intros.
+    split;intros;auto.
+    destruct H0. subst.
+    subst;auto.
+  Qed.
+
+  Lemma config_refinement_bind : forall (c1 :program Σ A) (c2: A -> program Σ B) (σ1 σ2: Σ) a ,
+    c1 σ1 a σ2 ->
+    (σ1, bind c1 c2 ) ↪ ( σ2, c2 a).
+  Proof.
+    intros; unfold config_refinement; unfold_monad; simpl; sets_unfold; intros.
+    eexists;eauto.
+  Qed.
+  
+  Theorem configrefine_decompose (c1 c2: program Σ A) (st1 st2: Σ):
+    (st1, c1) ↪  (st2, c2) <->
+    (forall X, st1 ∈ weakestpre c1 X -> st2 ∈ weakestpre c2 X).
+  Proof.
+    split;intros.
+    - unfold config_refinement, weakestpre in *.
+      sets_unfold. sets_unfold in H0.
+      intros. eapply H0;auto.
+    - specialize (H (fun r st3 => c1 st1 r st3)).
+      unfold config_refinement, weakestpre in *.
+      sets_unfold in H.
+      intros. apply H;auto.
+  Qed. 
+
+End config_refinement_rules.
+End ConfigReineStatreRelMonad.
+
+
+Module RelHoareNormalDenoAsbMonad.
+Export ConfigReineStatreRelMonad.
+Export normaldeno.
+
+Definition valid_quadruples {Σₗ Σₕ A: Type} (P: @binasrt Σₗ Σₕ ) (cₗ: denosem) (cₕ: program Σₕ A) (Q: A -> @binasrt Σₗ Σₕ) :=
+  forall st1 st1', P (st1, st1') -> 
+  forall st2, cₗ.(nrm) st1 st2 -> 
+  (exists st2' a, cₕ st1' a st2' /\ Q a (st2, st2') ).
+
+(* Alternative Definition of Relational Hoare Triples *)
+Definition valid_RelTriples {Σₗ Σₕ A: Type} (P: @relasrt Σₗ Σₕ (program Σₕ A)) (cₗ: @denosem Σₗ) (Q: @relasrt Σₗ Σₕ (program Σₕ A)) :=
+  forall st1 st1' (cₕ: (program Σₕ A)) , P (st1, st1', cₕ) -> 
+  forall st2, cₗ.(nrm) st1 st2 -> ( exists st2' cₕ', ( st1', cₕ ) ↪ ( st2', cₕ' ) /\ Q (st2, st2', cₕ')).
+
+Notation " '⊢' '{{' P '}}' cₗ '≾' cₕ '{{' Q '}}'" := (valid_quadruples P cₗ cₕ Q) (at level 71, no associativity).
+Notation " '⊢' '⟨' P '⟩' c '⟨' Q '⟩'" := (valid_RelTriples P c Q) (at level 71, no associativity).
+
+
+Section reltriple_correct.
+  Context {Σₗ Σₕ: Type}.
+  Import MonadNotation.
+  Local Open Scope monad.
+  Local Open Scope asrt_scope.
+
+Lemma quadruple2reltriple {A: Type}: forall (P: @binasrt Σₗ Σₕ ) (cₗ: (@denosem Σₗ))  (cₕ: program Σₕ A)  (Q : A -> @binasrt Σₗ Σₕ),
+    ⊢ {{P}} cₗ ≾ cₕ {{Q}} <-> ⊢ ⟨ ↑ P && [cₕ ]ₕ ⟩ cₗ ⟨ EX r : A, ↑ (Q r) && [ret r]ₕ  ⟩.
+  Proof.
+    intros;split.
+    - unfold valid_RelTriples, valid_quadruples.
+      unfold lift, exp, andp, Aspec.
+      intros HQ lst1 hst1 cₕ' [HP ?].
+      subst.
+      intros lst2 Hleval.
+      specialize (HQ _ _ HP _ Hleval) as (hst2 & a & Hheval & HQ).
+      do 2 eexists.
+      split;eauto.
+      unfold config_refinement.
+      intros.
+      unfold ret in H. destruct H. subst.
+      auto.
+    - unfold valid_RelTriples, valid_quadruples, lift.
+      unfold lift, exp, andp, Aspec.
+      intros HT lst1 hst1 HP.
+      intros lst2 Hleval.
+      specialize (HT lst1 hst1 _ (ltac:(split;auto)) _ Hleval) as (hst2 & ? & Hheval & a &  HQ & ?).
+      subst.
+      do 2 eexists.
+      split;eauto.
+      eapply Hheval.
+      unfold_monad.  auto.
+  Qed.
+
+End reltriple_correct.
+
+End RelHoareNormalDenoAsbMonad.
+
+
+
+(* low -level use part of practical deno *)
+Module RelHoareNormalDenoAsbMonad2.
+Export ConfigReineStatreRelMonad.
+Export practicaldeno.
+
+Definition valid_quadruples {Σₗ Σₕ A: Type} (P: @binasrt Σₗ Σₕ ) (cₗ: denosem) (cₕ: program Σₕ A) (Q: A -> @binasrt Σₗ Σₕ) :=
+  forall st1 st1', P (st1, st1') -> 
+  forall st2, cₗ.(nrm) st1 st2 -> 
+  (exists st2' a, cₕ st1' a st2' /\ Q a (st2, st2') ).
+
+(* Alternative Definition of Relational Hoare Triples *)
+Definition valid_RelTriples {Σₗ Σₕ A: Type} (P: @relasrt Σₗ Σₕ (program Σₕ A)) (cₗ: @denosem Σₗ) (Q: @relasrt Σₗ Σₕ (program Σₕ A)) :=
+  forall st1 st1' (cₕ: (program Σₕ A)) , P (st1, st1', cₕ) -> 
+  forall st2, cₗ.(nrm) st1 st2 -> ( exists st2' cₕ', ( st1', cₕ ) ↪ ( st2', cₕ' ) /\ Q (st2, st2', cₕ')).
+
+Notation " '⊢' '{{' P '}}' cₗ '≾' cₕ '{{' Q '}}'" := (valid_quadruples P cₗ cₕ Q) (at level 71, no associativity).
+Notation " '⊢' '⟨' P '⟩' c '⟨' Q '⟩'" := (valid_RelTriples P c Q) (at level 71, no associativity).
+
+
+Section reltriple_correct.
+  Context {Σₗ Σₕ: Type}.
+  Import MonadNotation.
+  Local Open Scope monad.
+  Local Open Scope asrt_scope.
+
+Lemma quadruple2reltriple {A: Type}: forall (P: @binasrt Σₗ Σₕ ) (cₗ: (@denosem Σₗ))  (cₕ: program Σₕ A)  (Q : A -> @binasrt Σₗ Σₕ),
+    ⊢ {{P}} cₗ ≾ cₕ {{Q}} <-> ⊢ ⟨ ↑ P && [cₕ ]ₕ ⟩ cₗ ⟨ EX r : A, ↑ (Q r) && [ret r]ₕ  ⟩.
+  Proof.
+    intros;split.
+    - unfold valid_RelTriples, valid_quadruples.
+      unfold lift, exp, andp, Aspec.
+      intros HQ lst1 hst1 cₕ' [HP ?].
+      subst.
+      intros lst2 Hleval.
+      specialize (HQ _ _ HP _ Hleval) as (hst2 & a & Hheval & HQ).
+      do 2 eexists.
+      split;eauto.
+      unfold config_refinement.
+      intros.
+      unfold ret in H. destruct H. subst.
+      auto.
+    - unfold valid_RelTriples, valid_quadruples, lift.
+      unfold lift, exp, andp, Aspec.
+      intros HT lst1 hst1 HP.
+      intros lst2 Hleval.
+      specialize (HT lst1 hst1 _ (ltac:(split;auto)) _ Hleval) as (hst2 & ? & Hheval & a &  HQ & ?).
+      subst.
+      do 2 eexists.
+      split;eauto.
+      eapply Hheval.
+      unfold_monad.  auto.
+  Qed.
+
+End reltriple_correct.
+
+End RelHoareNormalDenoAsbMonad2.
