EncRelSeq/MonadsAsHigh/AbsMonadE/encrel.v
@@ -1,0 +1,243 @@
+From SetsClass Require Import SetsClass.
+Require Import MonadLib.MonadLib.
+Import StateRelMonadErr.
+From EncRelSeq.Basics Require Import semantics basicasrt relasrt encdefs.
+From EncRelSeq.UBError Require Import errsem hoarelogic encrel.
+From EncRelSeq.MonadsAsHigh.AbsMonadE Require Import relhoarelogic.
+
+Require Import Coq.Logic.Classical_Prop.
+
+Module EncPracticalDenoAbsMonad.
+Import practicaldeno.
+Import HoarePracticalDeno.
+Import RelHoarePracticalDenoAsbMonad.
+
+Definition valid_reltriple {Σₗ Σₕ A: Type}:= valid_relT Σₗ Σₕ (@denosem Σₗ) (program Σₕ A) (A -> Σₕ -> Prop).
+
+Notation " '⊢ₑ' '⟨' P '⟩' c '⟨' Q '⟩'" := (valid_reltriple P c Q) (at level 71, no associativity).
+
+Local Open Scope asrt_scope.
+
+Import MonadNotation.
+Local Open Scope monad.
+Local Open Scope asrt_scope.
+Section normal_validity_soundness.
+  Context {Σₗ Σₕ: Type}.
+
+  Theorem encoding_correctness : forall {A: Type} (P: @relasrt Σₗ Σₕ (program Σₕ A)) (cₗ: denosem)  (Q :  @relasrt Σₗ Σₕ (program Σₕ A)),
+    ⊢ ⟨ P ⟩ cₗ ⟨ Q ⟩ <-> ⊢ₑ ⟨ P ⟩ cₗ ⟨ Q ⟩.
+  Proof.
+    unfold valid_reltriple, valid_relT; simpl_ldefs;simpl_hdefs.
+    intros;split.
+    - unfold valid_RelTriples, valid_triple.
+      intros HT X st1 HP.
+      unfold encode_asrt in *. simpl_hdefs.
+      destruct HP as (σₕ & cₕ & [Hherr Hhnrm] & HP).
+      specialize (HT _ _ _ HP) as [Herr Hnrm].
+      split.
+      + unfold not. intros.
+        apply Hherr. apply Herr. auto.
+      + 
+      intros st2 Heval.
+      unfold encode_asrt.
+      specialize (Hnrm _ Heval) as [ | (σₕ' & cₕ' &  Hheval  & HQ)];[ contradiction | ].
+      do 2 eexists. split;[ | eauto].
+      destruct Hheval as [Hheval1 Hheval2].
+      unfold MonadErrHoare.weakestpre in *.
+      sets_unfold.
+      split.
+      * intros ?. eapply Hherr. eapply Hheval2. eauto.
+      * intros.
+      eapply Hhnrm;eauto. sets_unfold. auto.
+    - unfold valid_RelTriples, valid_triple.
+      intros HT st1 σₕ cₕ HP.
+      specialize (HT (fun r x => cₕ.(nrm) σₕ r x) st1).
+      split.
+      + intros. 
+        pose proof classic (cₕ.(err) σₕ) as [ | ];[auto | ].
+        assert (([|P|](fun (r : A) (x : Σₕ) => cₕ.(nrm) σₕ r x)) st1).
+        { unfold encode_asrt. simpl_hdefs.
+          do 2 eexists. split;[ | eauto].
+          unfold MonadErrHoare.weakestpre; sets_unfold. auto. 
+        }
+        specialize (HT H1) as [? _].
+        contradiction.
+      + intros lst2 Hleval.
+        pose proof classic (cₕ.(err) σₕ) as [ | ];[auto | ].
+        assert (([|P|](fun (r : A) (x : Σₕ) => cₕ.(nrm) σₕ r x)) st1).
+        { unfold encode_asrt. simpl_hdefs.
+          do 2 eexists. split;[ | eauto].
+          unfold MonadErrHoare.weakestpre; sets_unfold. auto. 
+        }
+        specialize (HT H0) as [_ HT].
+        specialize (HT _ Hleval).
+        destruct HT as [σₕ' [cₕ' [? ?]]];subst.
+        right.
+        do 2 eexists.
+        split;eauto.
+        destruct H1.
+        unfold config_refinement.
+        split.
+        * intros.
+          eapply H3;eauto.
+        * intros.
+          contradiction. 
+  Qed. 
+
+  Theorem validity_conrrectness : forall {A: Type} (P: @binasrt Σₗ Σₕ ) (cₗ: denosem)  (cₕ: program Σₕ A)  (Q : A -> @binasrt Σₗ Σₕ),
+    ⊢ {{P}} cₗ ≾ cₕ {{Q}} <-> ⊢ₑ ⟨ ↑ P && [cₕ ]ₕ ⟩ cₗ ⟨ EX r : A, ↑ (Q r) && [ret r]ₕ ⟩.
+  Proof.
+    intros.
+    split;intros.
+    eapply encoding_correctness.
+    eapply quadruple2reltriple;auto.
+
+    eapply quadruple2reltriple.
+    eapply encoding_correctness;auto.
+  Qed.
+
+End normal_validity_soundness.
+End EncPracticalDenoAbsMonad.
+
+
+Module PracticalDenoAbsMonadEncRules.
+
+Import practicaldeno.
+Import EncPracticalDenoAbsMonad.
+
+Local Open Scope asrt_scope. 
+
+(**********************************************************************************)
+(*   encoded hoare rules                                                          *)
+(**********************************************************************************)
+
+Import HoarePracticalDeno PracticalDenoConstructs.
+Import HoarePracticalDenoRules.
+Import RelHoarePracticalDenoAsbMonad.
+
+
+  Section  encrules.
+  Context {Σₗ Σₕ: Type}.
+  Ltac destructs H := rel_destruct Σₗ Σₕ (@denosem Σₕ) (@denosem Σₗ) H.
+
+
+
+(**********************************************************************************)
+(*    trans reltriple into hoare triple                                           *)
+(**********************************************************************************)
+
+  Lemma  reltriple_triple_equiv1 {A:Type}: forall (P: @asrt Σₗ) Ps (s: program Σₕ A) c Q,
+    ⊢ ⟨ ⌊ P ⌋ && ⌈ Ps ⌉ && [ s ]ₕ ⟩ c ⟨ Q ⟩ <->
+    (forall X, ⊢∀ {{!! Exec Ps s X && P}} c {{[|Q|](X)}}).
+  Proof.
+    intros;split.
+    - intros. apply encoding_correctness in H.
+    specialize (H X). simpl_ldefs.
+    eapply hoare_conseq;eauto.
+    apply (logic_equiv_derivable1_2 (encode_decomposed X P Ps s)).
+    cbv. auto.
+    - intros. apply encoding_correctness.
+      unfold valid_reltriple, valid_relT; intros.
+      specialize (H X).
+      eapply hoare_conseq;eauto.
+      apply (logic_equiv_derivable1_1 (encode_decomposed X P Ps s)).
+      cbv. auto.
+  Qed.
+
+  Lemma  reltriple_triple_equiv {A R: Type}: forall (P: @asrt Σₗ) Ps (s: program Σₕ R) c B Q Ps',
+    ⊢ ⟨ ⌊ P ⌋ && ⌈ Ps ⌉ && [ s ]ₕ ⟩ c ⟨EX (r: R) (a:A), !! (B a r) && ⌊ Q a r ⌋ && ⌈ Ps' a r⌉ && [ ret r ]ₕ ⟩ <->
+    (forall X : R -> Σₕ -> Prop,
+    ⊢∀ {{!! Exec Ps s X && P}} c {{EX r a, !! Exec (Ps' a r) (ret r) X && !! (B a r) && (Q a r)}}).
+  Proof.
+    intros;split.
+    - intros.
+      apply encoding_correctness in H.
+    specialize (H X).  simpl_ldefs. 
+    eapply hoare_conseq;eauto.
+    eapply (logic_equiv_derivable1_2 (encode_decomposed X P Ps s)).
+    apply logic_equiv_derivable1_1.
+    eapply logic_equiv_trans.
+    apply logic_equiv_symm; apply (encode_exp_equiv _ _ ).
+    apply ex_logic_euiqv_elim_both;intros r.
+    apply encode_normal_form.
+    - intros. apply encoding_correctness.
+      unfold valid_reltriple, valid_relT; intros.
+      specialize (H X). 
+      eapply hoare_conseq;eauto.
+      apply (logic_equiv_derivable1_1 (encode_decomposed X P Ps s)).
+      apply logic_equiv_derivable1_2.
+      eapply logic_equiv_trans.
+      apply logic_equiv_symm; apply (encode_exp_equiv _ _ ).
+      apply ex_logic_euiqv_elim_both;intros r.
+      apply encode_normal_form.
+  Qed.
+
+  
+  Lemma high_focus_as_conseqpre {A B: Type} (cₗ: @denosem Σₗ) (cₕ1: program Σₕ A) (cₕ2: A -> program Σₕ B) F P R Q:
+    forall X a,
+    MonadErrHoare.valid_angelic_triple P cₕ1 (fun r σ => r = a /\ R σ) ->
+    ⊢∀ {{!! Exec R (cₕ2 a) X && F}} cₗ {{[|Q|](X)}} ->
+    ⊢∀ {{!! Exec P (bind cₕ1 cₕ2) X && F}} cₗ {{[|Q|](X)}}.
+  Proof.
+    intros.
+    eapply hoare_conseq_pre;[ | eauto].
+    apply derivable1_andp_mono;[ | reflexivity].
+    apply coq_prop_imply.
+    eapply highstepbind_derive.
+    eapply hs_eval_equiv_angelic_triple;auto.
+  Qed.
+
+  Lemma low_focus_as_seq {A: Type}  (cₗ1 cₗ2: @denosem Σₗ) (cₕ:  program Σₕ A) F P R Q:
+    forall X,
+    ⊢∀ {{P}} cₗ1 {{R}}  ->
+    ⊢∀ {{!! Exec F cₕ X && R}} cₗ2 {{[|Q|](X)}} ->
+    ⊢∀ {{!! Exec F cₕ X && P}} (seq cₗ1 cₗ2) {{[|Q|](X)}}.
+  Proof.
+    intros.
+    eapply hoare_Seq;eauto.
+    eapply hoare_coqprop_preintro.
+    intros.
+    eapply hoare_coqprop_postintro;auto.
+  Qed.
+
+End encrules.
+
+
+Section composition_rules.
+
+Lemma comp_fc_as_conseq {Σₗ Σₕ A: Type}:forall 
+  (P: @binasrt Σₗ Σₕ) (cₗ: denosem) (cₕ: program Σₕ A) (Q: A -> @binasrt Σₗ Σₕ) (Pₕ: @asrt Σₕ) Qₕ,
+  ((forall X, ⊢∀ {{ [|↑ P && [cₕ ]ₕ|](X) }} cₗ {{ [|EX a, ↑ Q a && [ret a ]ₕ|](X) }})) -> 
+  MonadErrHoare.Hoare Pₕ cₕ Qₕ ->
+  ⊢∀ {{ P ⋈_π Pₕ }} cₗ {{ EX a, (Q a) ⋈_π (Qₕ a) }}.
+Proof.
+  intros * HRT HHT.
+  eapply hoare_conseq_pre.  
+  { apply (logic_equiv_derivable1_2 (comp_proj_equiv _ _ )). }
+  eapply hoare_exists_intro; intros σₕ.
+  eapply hoare_coqprop_preintro. intros HPH.
+  specialize (HRT (fun r (x: Σₕ) => cₕ.(nrm) σₕ r x)).
+  eapply hoare_conseq;eauto.
+  - intros st1 ?.
+    unfold encode_asrt, lift, basicasrt.andp, Aspec. simpl.
+    do 2 eexists. split;[ | eauto].
+    unfold MonadErrHoare.weakestpre.
+    destruct HHT.
+    specialize (H1 _ HPH).
+    split;auto.
+  - intros st1 HQ.
+    unfold encode_asrt, lift, basicasrt.andp, Aspec in HQ.
+    destruct HQ as [σₕ' [cₕ' [? [? [? ?]]]]]. subst. simpl_hdefs.
+    unfold MonadErrHoare.weakestpre in H. sets_unfold in H.
+    destruct H.
+    specialize (H1 x σₕ' (ltac:(unfold_monad;auto))).
+    destruct HHT. 
+    specialize (H2 _ _ _ HPH H1).
+    exists x.
+    do 2 eexists. cbv. split;eauto.
+Qed.
+
+
+End  composition_rules.
+End PracticalDenoAbsMonadEncRules.
+
