EncRelSeq/MonadsAsHigh/AbsMonadE/relhoarelogic.v
@@ -1,0 +1,139 @@
+Require Import Coq.Classes.RelationClasses.
+From SetsClass Require Import SetsClass.
+Require Import MonadLib.MonadLib.
+Import StateRelMonadErr.
+From EncRelSeq.Basics Require Import basicasrt relasrt.
+From EncRelSeq Require Export semantics errsem.
+
+Local Open Scope sets_scope.
+
+Ltac any_nrm x ::=
+  match type of x with
+  | practicaldeno.denosem => exact (practicaldeno.nrm x)
+  | program _ _ => exact (MonadErr.nrm x)
+  end.
+
+
+Ltac any_err x ::=
+  match type of x with
+  | practicaldeno.denosem => exact (practicaldeno.err x)
+  | program _ _ => exact (MonadErr.err x)
+  end.
+
+Module ConfigReineStatreRelMonadErr.
+
+(* Configuration Refinement *)
+Definition config_refinement {Σ A: Type} (g1 g2: (Σ * program Σ A)%type ) : Prop :=
+  let '(σ1, c1) := g1 in
+  let '(σ2, c2) := g2 in
+  (forall r σ₃, c2.(nrm) σ2 r σ₃ -> c1.(nrm) σ1 r σ₃) /\ 
+  (c2.(err) σ2 -> c1.(err) σ1 ).
+
+Arguments config_refinement: simpl never.
+Notation " g1 '↪' g2 " := (config_refinement g1 g2) (at level 28, left associativity).
+
+#[export] Instance configrefine_reflexivity {Σ A: Type}: Reflexive (@config_refinement Σ A).
+Proof.
+  hnf. unfold config_refinement. intros. intuition eauto. Qed. 
+#[export] Instance configrefine_refinement_transivity {Σ A: Type}: Transitive (@config_refinement Σ A).
+Proof.
+  hnf. unfold config_refinement. intros [? ?] [? ?] [? ?]. intuition eauto. Qed. 
+
+
+Section config_refinement_rules.
+  Context {Σ A B: Type}.
+
+  Import MonadNotation.
+  Local Open Scope monad.
+
+  Lemma config_refinement_ret : forall (c: program Σ A) (σ1 σ2: Σ) a,
+    c.(nrm) σ1 a σ2 <->
+    ( σ1, c ) ↪ ( σ2, ret a).
+  Proof.
+    intros; unfold config_refinement; simpl; unfold_monad; sets_unfold; intros.
+    split;intros.
+    - split. intros. destruct H0. subst;auto.
+      tauto.
+    - destruct H. auto.
+  Qed.
+
+  Lemma config_refinement_bind : forall (c1 :program Σ A) (c2: A -> program Σ B) (σ1 σ2: Σ) a ,
+    c1.(nrm) σ1 a σ2 ->
+    (σ1, bind c1 c2 ) ↪ ( σ2, c2 a).
+  Proof.
+    intros; unfold config_refinement; unfold_monad; simpl; sets_unfold; intros.
+    split;intros.
+    - eexists;eauto.
+    - right.
+    eexists;eauto.
+  Qed.
+  
+End config_refinement_rules.
+End ConfigReineStatreRelMonadErr.
+
+
+Module RelHoarePracticalDenoAsbMonad.
+Export ConfigReineStatreRelMonadErr.
+Export practicaldeno.
+
+
+
+Definition valid_quadruples {Σₗ Σₕ A: Type} (P: @binasrt Σₗ Σₕ ) (cₗ: denosem) (cₕ: program Σₕ A) (Q: A -> @binasrt Σₗ Σₕ) :=
+  forall st1 st1', P (st1, st1') -> (cₗ.(err) st1 -> cₕ.(err) st1')  /\
+  forall st2, cₗ.(nrm) st1 st2 -> (cₕ.(err) st1' \/ 
+  (exists st2' a, cₕ.(nrm) st1' a st2' /\ Q a (st2, st2') )).
+
+(* Alternative Definition of Relational Hoare Triples *)
+Definition valid_RelTriples {Σₗ Σₕ A: Type} (P: @relasrt Σₗ Σₕ (program Σₕ A)) (cₗ: @denosem Σₗ) (Q: @relasrt Σₗ Σₕ (program Σₕ A)) :=
+  forall st1 st1' (cₕ: (program Σₕ A)) , P (st1, st1', cₕ) ->  (cₗ.(err) st1 -> cₕ.(err) st1') /\
+  forall st2, cₗ.(nrm) st1 st2 -> (cₕ.(err) st1' \/ ( exists st2' cₕ', ( st1', cₕ ) ↪ ( st2', cₕ' ) /\ Q (st2, st2', cₕ'))).
+
+Notation " '⊢' '{{' P '}}' cₗ '≾' cₕ '{{' Q '}}'" := (valid_quadruples P cₗ cₕ Q) (at level 71, no associativity).
+Notation " '⊢' '⟨' P '⟩' c '⟨' Q '⟩'" := (valid_RelTriples P c Q) (at level 71, no associativity).
+
+Section reltriple_correct.
+  Context {Σₗ Σₕ: Type}.
+  Import MonadNotation.
+  Local Open Scope monad.
+  Local Open Scope asrt_scope.
+
+  Lemma quadruple2reltriple {A: Type}: forall (P: @binasrt Σₗ Σₕ ) (cₗ: (@denosem Σₗ))  (cₕ: program Σₕ A)  (Q : A -> @binasrt Σₗ Σₕ),
+    ⊢ {{P}} cₗ ≾ cₕ {{Q}} <-> ⊢ ⟨ ↑ P && [cₕ ]ₕ ⟩ cₗ ⟨ EX r : A, ↑ (Q r) && [ret r]ₕ  ⟩.
+  Proof.
+    intros;split.
+    - unfold valid_RelTriples, valid_quadruples.
+      unfold lift, exp, andp, Aspec.
+      intros HQ lst1 hst1 cₕ' [HP ?].
+      subst.
+      specialize (HQ _ _ HP) as [HQerr HQnrm].
+      split;[auto | ].
+      intros lst2 Hleval.
+      specialize (HQnrm _ Hleval) as [ | (hst2 & a & Hheval & HQ)];[auto | right].
+      unfold lift, exp.
+      do 2 eexists.
+      split;eauto.
+      unfold config_refinement.
+      split.
+      { intros.
+      unfold ret in H. destruct H. subst.
+      auto. }
+      intros.
+      unfold ret in H. cbn in H. sets_unfold in H. contradiction.
+    - unfold valid_RelTriples, valid_quadruples, lift.
+      unfold lift, exp, andp, Aspec.
+      intros HT lst1 hst1 HP.
+      specialize (HT lst1 hst1 _ (ltac:(split;auto))) as [HTerr HTnrm].
+      split;[auto | ].
+      intros lst2 Hleval.
+      specialize (HTnrm _ Hleval) as [ | (hst2 & ? & Hheval & a &  HQ & ?)];[auto | right].
+      subst.
+      do 2 eexists.
+      split;eauto.
+      eapply Hheval.
+      unfold ret. cbn. auto.
+  Qed.
+
+End reltriple_correct.
+
+End RelHoarePracticalDenoAsbMonad.
+
